FRACTRAN computable relations are functional

theories/FRACTRAN/Utils/FRACTRAN_computable.v
@@ -2,6 +2,7 @@ Require Import Undecidability.FRACTRAN.FRACTRAN.
 
 From Coq Require Import List Vector Nat.
 Import ListNotations Vector.VectorNotations.
+From Undecidability Require Import Utils.prime FRACTRAN_sss Code.sss fractran_utils.
 
 Fixpoint enc {k} p i (v : Vector.t nat k) : nat := 
   match v with
@@ -10,7 +11,20 @@ Fixpoint enc {k} p i (v : Vector.t nat k) : nat :=
   end.
 
 Definition FRACTRAN_computable {k} (p : nat -> nat) (R : Vector.t nat k -> nat -> Prop) := 
-  exists P : list (nat * nat), 
+  exists P : list (nat * nat), fractran_regular P /\
     forall v : Vector.t nat k,
-      (forall m, R v m <-> fractran_eval P (enc p 1 v) (p 0))
+      (forall m, R v m <-> fractran_eval P (enc p 1 v) ((p 0)^m))
     /\ (forall n, fractran_eval P (enc p 1 v) n -> exists m, n = (p 0) ^ m).
+
+Lemma FRACTRAN_computable_functional {k} (p : nat -> nat) (R : Vector.t nat k -> nat -> Prop) :
+  (forall i j, p i = p j -> i = j) ->
+  (forall i, prime (p i)) ->
+  FRACTRAN_computable p R -> forall v m1 m2, R v m1 -> R v m2 -> m1 = m2.
+Proof.
+  intros Hpf Hpp (P & Hreg & HP) v m1 m2 H1 % HP H2 % HP. 
+  eapply eval_iff in H1 as [H1 H1'], H2 as [H2 H2'].
+  assert (p 0 ^ m1 = p 0 ^ m2).
+  - eapply fractran_compute_fun; eauto.
+  - assert (prime (p 0)) as ? % prime_ge_2 by eauto.
+    eapply PeanoNat.Nat.pow_inj_r; try eassumption.
+Qed.
